InferMatch.v
@@ -1,0 +1,109 @@
+Require Import Coq.Strings.String.
+
+Require Export SystemFR.StepTactics.
+Require Export SystemFR.ErasedRecGen.
+Require Export SystemFR.ErasedSingleton.
+
+Opaque reducible_values.
+
+Lemma evaluate_list_match:
+  forall ρ v t2 t3,
+    valid_interpretation ρ ->
+    wf t2 0 ->
+    wf t3 2 ->
+    is_erased_term t2 ->
+    is_erased_term t3 ->
+    pfv t2 term_var = nil ->
+    pfv t3 term_var = nil ->
+    [ ρ | v : List ]v -> (
+      (v = tnil /\ star scbv_step (list_match v t2 t3) t2) \/
+      (exists h l,
+         v = tcons h l /\
+         [ list_match v t2 t3 ≡ open 0 (open 1 t3 h) l ]
+      )
+    ).
+Proof.
+  unfold List, list_match.
+  intros.
+  apply (reducible_values_unfold_gen _ _ _ _ 0) in H6;
+    repeat step || simp_spos || simp_red_top_level_hyp.
+
+  - left; steps; one_step.
+  - right; eexists; eexists; steps.
+    apply equivalent_trans with (open 0 (open 1 t3 (pi1 (pp a b))) (pi2 (pp a b))).
+    + equivalent_star;
+        eauto 3 with erased step_tactic;
+        eauto 3 with wf step_tactic;
+        try solve [ repeat apply pfv_shift_open || step ].
+
+      apply star_one.
+      eapply scbv_step_same.
+      apply SPBetaMatchRight; t_closer.
+      rewrite open_shift_open2; steps; t_closer;
+        eauto 3 with wf step_tactic.
+      rewrite no_shift_open; t_closer.
+      rewrite open_shift_open2; steps; t_closer;
+        eauto 3 with wf step_tactic.
+
+      2
+    eauto with smallstep.
+    apply Trans.
+    one_step.
+
+
+    open_none; auto.
+
+Opaque list_match.
+Opaque List_Match.
+
+  
+  
+  simp_red; steps.
+  
+
+  
+  intros.
+  unfold List
+  repeat step || simp_red.
+
+
+Lemma tmatch:
+  forall ρ t t2 t3 T2 T3,
+    [ ρ | t : List ] ->
+    [ ρ | t2 : T2 ] ->
+    (forall h t, [ ρ | h : T_top ] -> [ ρ | t : List ] ->
+            [ ρ | open 0 (open 1 t3 h) t : open 0 (open 1 T3 h) t ]) ->
+    [ ρ | list_match t t2 t3 : List_Match t T2 T3 ].
+Proof.
+Admitted.
+
+Lemma open_tmatch_helper:
+  forall Θ Γ t t2 t3 T2 T3 x1 x2,
+    ~ x1 ∈ support Γ ->
+    ~ x2 ∈ support Γ ->
+    [ Θ; Γ ⊨ t : List ] ->
+    [ Θ; Γ ⊨ t2 : T2 ] ->
+    [ Θ; (x1, T_top) :: (x2, List) :: Γ ⊨
+        open 0 (open 1 t3 (fvar x1 term_var)) (fvar x2 term_var) :
+        open 0 (open 1 T3 (fvar x1 term_var)) (fvar x2 term_var) ] ->
+    [ Θ; Γ ⊨ list_match t t2 t3 : List_Match t T2 T3 ].
+Proof.
+  unfold open_reducible;
+    repeat step || apply tmatch ||
+           rewrite substitute_list_match || rewrite substitute_List_Match;
+    eauto with wf.
+Admitted.
+
+Lemma open_tmatch:
+  forall Γ t t2 t3 T2 T3 x1 x2,
+    ~ x1 ∈ support Γ ->
+    ~ x2 ∈ support Γ ->
+    [ Γ ⊨ t : List ] ->
+    [ Γ ⊨ t2 : T2 ] ->
+    [ (x1, T_top) :: (x2, List) :: Γ ⊨
+        open 0 (open 1 t3 (fvar x1 term_var)) (fvar x2 term_var) :
+        open 0 (open 1 T3 (fvar x1 term_var)) (fvar x2 term_var) ] ->
+    [ Γ ⊨ list_match t t2 t3 : List_Match t T2 T3 ].
+Proof.
+  eauto using open_tmatch_helper.
+Qed.
