ScalaDepSugar.v
@@ -1,0 +1,161 @@
+Require Export SystemFR.ShiftOpen.
+
+Definition T_singleton T t :=
+  T_type_refine T (T_equiv (lvar 0 term_var) (shift 0 t 1)).
+
+Definition type_application T1 T2 : tree :=
+  T_type_refine T_top (
+    T_exists T1 (
+      T_exists T2 (
+        T_equiv (app (lvar 1 term_var) (lvar 0 term_var)) (lvar 2 term_var)
+      )
+    )
+  ).
+
+Definition List : tree :=
+  intersect
+    (T_sum T_top T_top)
+    (T_sum T_unit (T_prod T_top (lvar 0 type_var))).
+
+Definition tnil := tleft uu.
+Definition Nil := T_singleton List tnil.
+
+Definition Var x := T_singleton (fvar x term_var).
+
+Definition tcons h t := tright (pp h t).
+Definition Cons H T :=
+  T_exists H (T_exists T (
+    T_singleton List (tcons (lvar 1 term_var) (lvar 0 term_var))
+  )).
+
+Definition list_match t1 t2 t3 :=
+  sum_match t1 t2
+    (shift_open 0 (shift_open 1 t3 (pi1 (lvar 0 term_var))) (pi2 (lvar 0 term_var))).
+
+Definition List_Match t T2 T3 :=
+  T_union
+    (T_type_refine T2 (T_equiv t tnil))
+    (T_exists T_top (
+      (T_exists List (
+        (T_type_refine T3 (T_equiv t (tcons (lvar 2 term_var) (lvar 1 term_var))))
+      ))
+    )).
+
+Lemma substitute_list_match:
+  forall t1 t2 t3 l tag,
+    wfs l 0 ->
+    psubstitute (list_match t1 t2 t3) l tag =
+    list_match (psubstitute t1 l tag) (psubstitute t2 l tag) (psubstitute t3 l tag).
+Proof.
+  unfold list_match; repeat step || t_equality || rewrite substitute_shift_open.
+Qed.
+
+Lemma substitute_List_Match:
+  forall t1 t2 t3 l tag,
+    wfs l 0 ->
+    psubstitute (List_Match t1 t2 t3) l tag =
+    List_Match (psubstitute t1 l tag) (psubstitute t2 l tag) (psubstitute t3 l tag).
+Proof.
+  unfold list_match; repeat step || t_equality || rewrite substitute_shift_open.
+Qed.
+
+(*
+default: T
+def f: T = t[f]
+
+
+def f'(fuel): T =
+  if fuel == 0
+  then default
+  else t[f -> f'(fuel - 1)]
+
+val f = f'(globalFuel)
+
+*)
+
+Definition fix_default' t default fuel: tree :=
+  app
+    (notype_tfix ( (* unused and f *)
+      notype_lambda (           (* fuel *)
+        tmatch (lvar 0 term_var (* fuel *))
+          default
+          (shift_open 0 t
+            (app (lvar 2 term_var (* f *)) (lvar 0 term_var (* new fuel *)))
+          )
+        )
+      )
+    )
+    fuel
+.
+
+Parameter global_fuel: tree.
+Parameter is_nat_global_fuel: is_nat_value global_fuel.
+
+Definition fix_default t default := fix_default' t default global_fuel.
+
+Lemma wf_fix_default:
+  forall default t fuel,
+    wf t 1 ->
+    wf default 0 ->
+    wf fuel 0 ->
+    wf (fix_default' t default fuel) 0.
+Proof.
+  unfold fix_default;
+    repeat step;
+    eauto using wf_shift_open2 with wf step_tactic.
+Qed.
+
+Lemma subst_fix_default:
+  forall t default fuel l tag,
+    wfs l 0 ->
+    psubstitute (fix_default' t default fuel) l tag =
+    fix_default' (psubstitute t l tag) (psubstitute default l tag) (psubstitute fuel l tag).
+Proof.
+  unfold fix_default; repeat step || t_equality || rewrite substitute_shift_open in *.
+Qed.
+
+Lemma pfv_fix_default:
+  forall t default fuel tag,
+    pfv t tag = nil ->
+    pfv default tag = nil ->
+    pfv fuel tag = nil ->
+    pfv (fix_default' t default fuel) tag = nil.
+Proof.
+  repeat step || list_utils || rewrite pfv_shift_open.
+Qed.
+
+Lemma pfv_fix_default2:
+  forall t default fuel tag,
+    subset
+      (pfv (fix_default' t default fuel) tag)
+      (pfv t tag ++ pfv default tag ++ pfv fuel tag).
+Proof.
+  repeat step || list_utils || apply subset_union2; eauto with sets.
+  eapply subset_transitive; eauto using pfv_shift_open2; repeat step || sets; eauto with sets.
+Qed.
+
+Lemma is_erased_term_fix_default:
+  forall t default fuel,
+    is_erased_term t ->
+    is_erased_term default ->
+    is_erased_term fuel ->
+    is_erased_term (fix_default' t default fuel).
+Proof.
+  repeat step || apply is_erased_term_shift_open.
+Qed.
+
+Lemma is_erased_list: is_erased_type List.
+Proof. steps. Qed.
+
+Hint Resolve is_erased_list: erased.
+
+Lemma wf_list: forall k, wf List k.
+Proof. steps; eauto with lia. Qed.
+
+Hint Resolve wf_list: wf.
+
+Lemma open_list: forall k rep, open k List rep = List.
+Proof. steps. Qed.
+
+Lemma subst_list: forall l tag, psubstitute List l tag = List.
+Proof. steps. Qed.
